proof/crypto_scalarmult/curve25519/Curve25519_Hop4.ec
@@ -1,166 +1,153 @@
-require import AllCore Bool List Int (*IntExtra*) IntDiv CoreMap Real Zp.
+require import AllCore Bool List Int IntDiv CoreMap Real Zp25519.
 from Jasmin require import JModel.
+from JasminExtra require import JBigNum.
 require import Curve25519_Spec Curve25519_Hop1 Curve25519_Hop2 Curve25519_Hop3.
 
 require import Curve25519_smulx.
-import Curve25519_smulx.
 import Zp ZModpRing.
 require import Array4 Array8.
 
-(**FROM HERE**)
-require import W64limbs.
-
-(** representation : move to another file/use rep3/5 **)
-type Rep4 = W64.t Array4.t.
-op valRep4  (x : Rep4) : int = val_limbs64 (to_list x).
-op inzpRep4 (x : Rep4) : zp  = inzp (valRep4 x) axiomatized by inzpRep4E.
-abbrev zpcgrRep4 (x : Rep4) (z : int) : bool = zpcgr (valRep4 x) z.
-(** ************************************* **)
-
 (** step 0 : add sub mul sqr **)
-equiv eq_h4_add : MHop2.add ~ M._fe64_add_rrs:
-   f{1} = inzpRep4 f{2} /\
-   g{1} = inzpRep4 g{2}
+equiv eq_h4_add_rrs : MHop2.add ~ M.__add4_rrs:
+   ImplFpC f{1} f{2} /\
+   ImplFpC g{1} g{2}
     ==>
-   res{1} = inzpRep4 res{2}.
+   ImplFpC res{1} res{2}.
 proof.
 proc.
 admit.
 qed.
 
-equiv eq_h4_sub : MHop2.sub ~ M._fe64_sub_rrs:
-   f{1} = inzpRep4 f{2} /\
-   g{1} = inzpRep4 gs{2}
+equiv eq_h4_sub_rrs : MHop2.sub ~ M.__sub4_rrs:
+   ImplFpC f{1} f{2} /\
+   ImplFpC g{1} gs{2}
     ==>
-   res{1} = inzpRep4 res{2}.
+   ImplFpC res{1} res{2}.
 proof.
 proc.
 admit.
 qed.
 
-equiv eq_h4_mul_a24 : MHop2.mul_a24 ~ M._fe64_mul_a24:
-   f{1} = inzpRep4 fs{2} /\
+equiv eq_h4_mul_a24_rs : MHop2.mul_a24 ~ M.__mulx_mul4_a24_rs:
+   ImplFpC f{1} fs{2} /\
    a24{1} = to_uint a24{2}
     ==>
-   res{1} = inzpRep4 res{2}.
+   ImplFpC res{1} res{2}.
 proof.
 proc.
 admit.
 qed.
 
-equiv eq_h4_mul : MHop2.mul ~ M._fe64_mul_rsr:
-   f{1} = inzpRep4 fs{2} /\
-   g{1} = inzpRep4 g{2}
+equiv eq_h4_mul_rss : MHop2.mul ~ M.__mulx_mul4_rss:
+   ImplFpC f{1} fs{2} /\
+   ImplFpC g{1} gs{2}
     ==>
-   res{1} = inzpRep4 res{2}.
+   ImplFpC res{1} res{2}.
 proof.
 proc.
 admit.
 qed.
 
-equiv eq_h4_sqr : MHop2.sqr ~ M._fe64_sqr_rr:
-    f{1} = inzpRep4 f{2}
+equiv eq_h4_sqr_rr : MHop2.sqr ~ M.__mulx_sqr4_rr:
+    ImplFpC f{1} f{2}
     ==>
-    res{1} = inzpRep4 res{2}.
+    ImplFpC res{1} res{2}.
 proof.
 proc.
 admit.
 qed.
 
-(** step 0.5 : transitivity stuff **)
-equiv eq_h4_add_ssr : MHop2.add ~ M._fe64_add_ssr:
-   f{1} = inzpRep4 fs{2} /\
-   g{1} = inzpRep4 g{2}
+(** step 0.5 : transitivity **** **** **** **** *)
+
+(** add **)
+equiv eq_h4_add_ssr : MHop2.add ~ M.__add4_ssr:
+   ImplFpC f{1} fs{2} /\
+   ImplFpC g{1} g{2}
     ==>
-   res{1} = inzpRep4 res{2}.
+   ImplFpC res{1} res{2}.
 proof.
 proc.
 admit.
 qed.
 
-equiv eq_h4_add_sss : MHop2.add ~ M._fe64_add_sss:
-   f{1} = inzpRep4 fs{2} /\
-   g{1} = inzpRep4 gs{2}
+equiv eq_h4_add_sss : MHop2.add ~ M.__add4_sss:
+   ImplFpC f{1} fs{2} /\
+   ImplFpC g{1} gs{2}
     ==>
-   res{1} = inzpRep4 res{2}.
+   ImplFpC res{1} res{2}.
 proof.
 proc.
 admit.
 qed.
 
-equiv eq_h4_sub_ssr : MHop2.sub ~ M._fe64_sub_ssr:
-   f{1} = inzpRep4 fs{2} /\
-   g{1} = inzpRep4 g{2}
+(** sub **)
+equiv eq_h4_sub_ssr : MHop2.sub ~ M.__sub4_ssr:
+   ImplFpC f{1} fs{2} /\
+   ImplFpC g{1} g{2}
     ==>
-   res{1} = inzpRep4 res{2}.
+   ImplFpC res{1} res{2}.
 proof.
 proc.
 admit.
 qed.
 
-equiv eq_h4_sub_sss : MHop2.sub ~ M._fe64_sub_sss:
-   f{1} = inzpRep4 fs{2} /\
-   g{1} = inzpRep4 gs{2}
+equiv eq_h4_sub_sss : MHop2.sub ~ M.__sub4_sss:
+   ImplFpC f{1} fs{2} /\
+   ImplFpC g{1} gs{2}
     ==>
-   res{1} = inzpRep4 res{2}.
+   ImplFpC res{1} res{2}.
 proof.
 proc.
 admit.
 qed.
 
-equiv eq_h4_mul_a24_ss : MHop2.mul_a24 ~ M._fe64_mul_a24_ss:
-   f{1} = inzpRep4 fs{2} /\
+(** mul a24 **)
+equiv eq_h4_mul_a24_ss : MHop2.mul_a24 ~ M.__mulx_mul4_a24_ss:
+   ImplFpC f{1} fs{2} /\
    a24{1} = to_uint a24{2}
     ==>
-   res{1} = inzpRep4 res{2}.
+   ImplFpC res{1} res{2}.
 proof.
 proc.
 admit.
 qed.
 
-equiv eq_h4_mul_rss : MHop2.mul ~ M._fe64_mul_rss:
-   f{1} = inzpRep4 fs{2} /\
-   g{1} = inzpRep4 gs{2}
+(** mul **)
+equiv eq_h4_mul_ssr : MHop2.mul ~ M.__mulx_mul4_ssr:
+   ImplFpC f{1} fs{2} /\
+   ImplFpC g{1} g{2}
     ==>
-   res{1} = inzpRep4 res{2}.
+   ImplFpC res{1} res{2}.
 proof.
 proc.
 admit.
 qed.
 
-equiv eq_h4_mul_ssr : MHop2.mul ~ M._fe64_mul_ssr:
-   f{1} = inzpRep4 fs{2} /\
-   g{1} = inzpRep4 g{2}
+equiv eq_h4_mul_sss : MHop2.mul ~ M.__mulx_mul4_sss:
+   ImplFpC f{1} fs{2} /\
+   ImplFpC g{1} gs{2}
     ==>
-   res{1} = inzpRep4 res{2}.
+   ImplFpC res{1} res{2}.
 proof.
 proc.
 admit.
 qed.
 
-equiv eq_h4_mul_sss : MHop2.mul ~ M._fe64_mul_sss:
-   f{1} = inzpRep4 fs{2} /\
-   g{1} = inzpRep4 gs{2}
+
+(** sqr **)
+equiv eq_h4_sqr_rs : MHop2.sqr ~ M.__mulx_sqr4_rs:
+    ImplFpC f{1} fs{2}
     ==>
-   res{1} = inzpRep4 res{2}.
+    ImplFpC res{1} res{2}.
 proof.
 proc.
 admit.
 qed.
 
-equiv eq_h4_sqr_rs : MHop2.sqr ~ M._fe64_sqr_rs:
-    f{1} = inzpRep4 fs{2}
+equiv eq_h4_sqr_ss : MHop2.sqr ~ M.__mulx_sqr4_ss:
+    ImplFpC f{1} fs{2}
     ==>
-    res{1} = inzpRep4 res{2}.
-proof.
-proc.
-admit.
-qed.
-
-equiv eq_h4_sqr_ss : MHop2.sqr ~ M._fe64_sqr_ss:
-    f{1} = inzpRep4 fs{2}
-    ==>
-    res{1} = inzpRep4 res{2}.
+    ImplFpC res{1} res{2}.
 proof.
 proc.
 admit.
@@ -168,7 +155,7 @@ qed.
 
 (** step 1 : decode_scalar_25519 **)
 equiv eq_h4_decode_scalar_25519 :
-  MHop2.decode_scalar_25519 ~ M.decode_scalar_25519:
+  MHop2.decode_scalar_25519 ~ M.__decode_scalar_25519_shl1:
   true ==> true.
 proof.
 admit.
@@ -176,38 +163,41 @@ qed.
 
 (** step 2 : decode_u_coordinate **)
 equiv eq_h4_decode_u_coordinate :
-  MHop2.decode_u_coordinate ~ M.decode_u_coordinate:
+  MHop2.decode_u_coordinate ~ M.__decode_u_coordinate:
   true ==> true.
 proof.
 admit.
 qed.
 
-(** step 3 : ith_bit **)
+(** step 3 : ith_bit **) (** TODO CHECKME : this should be handled before Hop4 **)
 equiv eq_h4_ith_bit :
-  MHop2.ith_bit ~ M.ith_bit:
+  MHop2.ith_bit ~ M.__next_bit:
   true ==> true.
 proof.
+proc.
 admit.
 qed.
 
 (** step 4 : cswap **)
 equiv eq_h4_cswap :
-  MHop2.cswap ~ M._fe64_cswap:
-  x2{1}         = inzpRep4 x2{2}  /\
-  z2{1}         = inzpRep4 z2r{2} /\
-  x3{1}         = inzpRep4 x3{2}  /\
-  z3{1}         = inzpRep4 z3{2}  /\
+  MHop2.cswap ~ M.__cswap4:
+  ImplFpC x2{1} x2{2}  /\
+  ImplFpC z2{1} z2r{2} /\
+  ImplFpC x3{1} x3{2}  /\
+  ImplFpC z3{1} z3{2}  /\
   b2i toswap{1} = to_uint toswap{2}
   ==>
-  res{1}.`1     = inzpRep4 res{2}.`1  /\
-  res{1}.`2     = inzpRep4 res{2}.`2  /\
-  res{1}.`3     = inzpRep4 res{2}.`3  /\
-  res{1}.`4     = inzpRep4 res{2}.`4.
+  ImplFpC res{1}.`1 res{2}.`1  /\
+  ImplFpC res{1}.`2 res{2}.`2  /\
+  ImplFpC res{1}.`3 res{2}.`3  /\
+  ImplFpC res{1}.`4 res{2}.`4.
 proof.
 proc.
 do 4! unroll for{2} ^while.
 case: (toswap{1}).
   rcondt {1} 1 => //. wp => /=; skip.
+    admit.
+(** TODO FROM HERE
     move => &1 &2 [#] 4!->> ??.
     have mask_set :  (set0_64.`6 - toswap{2}) = W64.onew. rewrite /set0_64 /=. smt(@W64).
     rewrite !mask_set /=.
@@ -225,21 +215,23 @@ case: (toswap{1}).
     have mask_not_set :  (set0_64.`6 - toswap{2}) = W64.zero. smt(@W64).
     rewrite !mask_not_set !andw0 !xorw0.
     smt(@Array4).
+**)
+  admit.
 qed.
 
 (** step 5 : add_and_double **)
 equiv eq_h4_add_and_double :
-  MHop2.add_and_double ~ M.add_and_double:
-  init{1} = inzpRep4 init{2} /\
-  x2{1}   = inzpRep4 x2{2}   /\
-  z2{1}   = inzpRep4 z2r{2}  /\
-  x3{1}   = inzpRep4 x3{2}   /\
-  z3{1}   = inzpRep4 z3{2}
+  MHop2.add_and_double ~ M.__add_and_double_mulx:
+  ImplFp  init{2} init{1} /\
+  ImplFpC x2{1} x2{2}     /\
+  ImplFpC z2{1} z2r{2}    /\
+  ImplFpC x3{1} x3{2}     /\
+  ImplFpC z3{1} z3{2}
   ==>
-  res{1}.`1 = inzpRep4 res{2}.`1 /\
-  res{1}.`2 = inzpRep4 res{2}.`2 /\
-  res{1}.`3 = inzpRep4 res{2}.`3 /\
-  res{1}.`4 = inzpRep4 res{2}.`4.
+  ImplFpC res{1}.`1 res{2}.`1 /\
+  ImplFpC res{1}.`2 res{2}.`2 /\
+  ImplFpC res{1}.`3 res{2}.`3 /\
+  ImplFpC res{1}.`4 res{2}.`4.
 proof.
 proc => /=.
   call eq_h4_mul_rss.
@@ -260,12 +252,12 @@ proc => /=.
   call eq_h4_sub_sss.
   call eq_h4_add_ssr.
   call eq_h4_sub_ssr.
-  wp. done.
+  wp. skip => /#.
 qed.
 
 (** step 6 : montgomery_ladder_step **)
 equiv eq_h4_montgomery_ladder_step :
- MHop2.montgomery_ladder_step ~ M.montgomery_ladder_step:
+ MHop2.montgomery_ladder_step ~ M.__montgomery_ladder_mulx:
  true ==> true.
 proof.
 admit.
@@ -273,7 +265,7 @@ qed.
 
 (** step 7 : montgomery_ladder **)
 equiv eq_h4_montgomery_ladder :
-  MHop2.montgomery_ladder ~ M.montgomery_ladder :
+  MHop2.montgomery_ladder ~ M.__montgomery_ladder_mulx :
   true ==> true.
 proof.
 admit.
@@ -281,14 +273,14 @@ qed.
 
 (** step 8 : iterated square **)
 equiv eq_h4_it_sqr :
- MHop2.it_sqr ~ M._fe64_it_sqr:
-   f{1}            =    inzpRep4 f{2} /\
+ MHop2.it_sqr ~ M.__mulx_it_sqr4_x2:
+   ImplFpC f{1} f{2}                  /\
    i{1}            =    to_uint i{2}  /\
    i{1}            <=   W64.modulus   /\
     2              <=   i{1}          /\
    i{1} %% 2        =   0
    ==>
-   res{1} = inzpRep4 res{2}.`2.
+   ImplFpC res{1} res{2}.`2.
 proof.
 proc.
   while (f{1}            =    inzpRep4 f{2}            /\ 
