proof/crypto_scalarmult/curve25519/Zp25519.ec
@@ -1,0 +1,479 @@
+require import Core Int Ring IntDiv StdOrder List.
+
+import Ring.IntID IntOrder.
+
+(*
+require import EClib.
+*)
+
+from Jasmin require import JModel.
+
+from JasminExtra require import JBigNum.
+
+require import Array4 Array8.
+
+abbrev nlimbs = 4.
+
+clone import BigNum as W64x4 with
+ op nlimbs <- nlimbs,
+ theory R.A <= Array4,
+ theory R2.A <= Array8
+ proof gt0_nlimbs by done.
+
+type R = W64.t Array4.t.
+type R2 = W64.t Array8.t.
+
+(* modular operations modulo P *)
+op P = 2^255 - 19 axiomatized by pE.
+
+axiom P_prime: prime P.
+
+lemma two_pow255E: 2^255 = 57896044618658097711785492504343953926634992332820282019728792003956564819968 by done.
+
+lemma pVal: P = 57896044618658097711785492504343953926634992332820282019728792003956564819949 by smt(pE two_pow255E).
+
+(* Embedding into ring theory *)
+require ZModP. (**** ****)
+clone import ZModP.ZModField as Zp with
+        op p <= P
+        rename "zmod" as "zp"
+        proof prime_p by exact P_prime.
+
+(* congruence "mod p" *)
+lemma zpcgr_over a b:
+ zpcgr (a + 2^255 * b) (a + 19 * b).
+proof.
+have /= ->: (2^ 255) = 19 + P by rewrite pE.
+by rewrite (mulzC _ b) mulzDr addzA modzMDr mulzC.
+qed.
+
+lemma inzp_over x:
+ inzp (2^255 * x) = inzp (19*x).
+proof. by have /= := zpcgr_over 0 x; rewrite -eq_inzp. qed.
+
+lemma twop255_cgr : 2^255 %% P = 19 by smt.
+lemma twop256_cgr : 2^256 %% P = 38 by smt.
+
+lemma P_cgr: (2^256 - 2^255 - 19)%%P = 0.
+proof.
+by rewrite -modzDml -(modzDm (2^256) (-2^255)) -modzNm
+     twop256_cgr twop255_cgr modzDmr /= modzDml.
+qed.
+
+lemma ltP_overflow x:
+ (x + 2^255 + 19 < 2^256) = (x < P).
+proof.
+have ->: 2^255 = P + 19 by rewrite pE /#. 
+have ->: 2^256 = P + P + 19 + 19 by rewrite !pE /#.
+smt().
+qed.
+
+op red x = if x + 2^255 + 19 < 2^256 then x else (x + 2^255 + 19) %% 2^256.
+
+lemma redE x:
+ P <= x < 2^256 =>
+ (x + 2^255 + 19) %% 2^256 = x - P.
+proof.
+move=> [H1 H2].
+pose y := x-P.
+rewrite (_: x= y+P) 1:/# (_:2^255 = P+19) 1:pE 1:/#.
+rewrite -addrA -addrA (_:P + (P + 19 + 19) = 2^256) 1:pE 1:/#.
+rewrite modzDr modz_small; last reflexivity.
+apply bound_abs.
+move: H2; have ->: 2^256 = P + P + 19 + 19 by rewrite !pE /#.
+smt(pVal).
+qed.
+
+lemma redP x:
+ 0 <= x < 2^256 =>
+ x %% P = red (red x).
+proof.
+move=> [H1 H2].
+rewrite /red !ltP_overflow.
+case: (x < P) => Hx1.
+ rewrite Hx1 /= modz_small; last done.
+ by apply bound_abs => /#.
+rewrite redE.
+ split => *; [smt() | assumption].
+case: (x - P < P) => Hx2.
+ rewrite {1}(_: x = x - P + P) 1:/# modzDr modz_small; last reflexivity.
+ by apply bound_abs => /#.
+rewrite redE.
+ split => *; first smt().
+ rewrite (_:W256.modulus = W256.modulus-0) 1:/#. 
+ apply (ltr_le_sub); first assumption. 
+ smt(pVal). 
+rewrite (_: x = x - P - P + P + P) 1:/#.
+rewrite modzDr modzDr modz_small.
+apply bound_abs; split => *; first smt().
+ move: H2; have ->: 2^256 = P + P + 19 + 19 by rewrite !pE /#.
+ smt(pVal).
+smt().
+qed.
+
+
+(** "Implements" relation *)
+(*abbrev ImplBool x y = (W64.to_uint x) = b2i y.*)
+abbrev ImplWord x y = W64.to_uint x = y.
+abbrev ImplZZ x y = valR x = y.
+abbrev ImplZZ2 x y = valR2 x = y.
+abbrev ImplFp x y = valR x = asint y.
+abbrev ImplFpC (y : zp , x : R (*W64.t Array4.t*)) : bool = zpcgr (asint y) (valR x).
+
+op pR: R = R.A.of_list 
+             W64.zero
+             [ W64.of_int 18446744073709551597
+             ; W64.of_int 18446744073709551615
+             ; W64.of_int 18446744073709551615
+             ; W64.of_int 9223372036854775807
+             ].
+
+lemma pRE: ImplZZ pR P.
+proof.
+by rewrite /pR R.bn2seq /= R.A.of_listK 1:/# /bn_seq pVal.
+qed.
+
+op zeroR : R = R.A.of_list W64.zero
+                 [ W64.zero; W64.zero; W64.zero; W64.zero ].
+
+lemma zeroRE: valR zeroR = 0.
+proof.
+by rewrite /zeroR R.bn2seq /= R.A.of_listK 1:/# /bn_seq.
+qed.
+
+
+abbrev M = 115792089237316195423570985008687907853269984665640564039457584007913129639936.
+
+op split256 x = (x %/ 2^256, x %% 2^256).
+
+op red256 (x: int) : int =
+ (split256 x).`2 + 38 * (split256 x).`1.
+
+lemma red256P x: zpcgr x (red256 x).
+proof.
+by rewrite {1}(divz_eq x (2^256)) -modzDml -modzMmr twop256_cgr 
+           modzDml /red256 /split256 /= addrC mulrC.
+qed.
+
+lemma red256_bnd B x:
+ 0 <= x < M * B => 
+ 0 <= red256 x < M + 38*B.
+proof.
+move=> [Hx1 Hx2]; rewrite /red256 /split256 /=; split => *.
+ apply addz_ge0; first smt(modz_cmp).
+ apply mulr_ge0; first done.
+ apply divz_ge0; smt().
+have H1: x %/ M < B by smt().
+have H2: x %% M < M by smt(modz_cmp).
+smt().
+qed.
+
+lemma red256_once x:
+ 0 <= x < M*M =>
+ 0 <= red256 x < M*39.
+proof.
+have ->: M*39 = M + 38*M by ring.
+exact red256_bnd.
+qed.
+
+lemma red256_twice x:
+ 0 <= x < M*M =>
+ 0 <= red256 (red256 x) < M*2.
+proof.
+move=> Hx; split => *.
+ smt(red256_once).
+move: (red256_once x Hx).
+move => Hy.
+move: (red256_bnd 39 _ Hy); smt().
+qed.
+
+lemma red256_twiceP x a b:
+ 0 <= x < M*M =>
+ (a,b) = split256 (red256 (red256 x)) =>
+(* 0 <= a < 2 /\ (a=0 \/ b <= 38*38).*)
+ a=0 \/ a=1 /\ b <= 38*38.
+proof.
+move=> Hx Hab.
+have Ha: 0 <= a < 2.
+ have H := (red256_twice x Hx).
+ move: Hab; rewrite /split256 => [[-> _]]; smt().
+case: (a=0) => Ea /=; first done.
+have {Ea} Ea: a=1 by smt().
+rewrite Ea /=.
+move: Hab; pose y := red256 x.
+rewrite /red256 /split256 /=.
+pose yL := y%%M.
+pose yH := y%/M.
+have Hy := red256_once x Hx.
+have HyH : 0 <= yH <= 38 by smt().
+move => [Hab1 Hab2].
+have E: M + b = yL + 38 * yH.
+ by move: (divz_eq (yL + 38 * yH) M); smt().
+smt(modz_cmp).
+qed.
+
+lemma red256_thrice x:
+ 0 <= x < M*M =>
+ 0 <= red256 (red256 (red256 x)) < M.
+proof.
+move=> Hx; pose y:= red256 (red256 x).
+rewrite /red256.
+have := (red256_twiceP x (split256 y).`1 (split256 y).`2 _ _).
+  smt(red256_twice).
+ smt().
+move=> [->|[-> H2]] /=.
+ rewrite /split256; smt(modz_cmp).
+split.
+ rewrite /split256; smt(modz_cmp).
+smt().
+qed.
+
+op reduce x = red256 (red256 (red256 x)).
+
+lemma reduceP x:
+ 0 <= x < M*M =>
+ zpcgr x (reduce x) /\ 0 <= reduce x < M.
+proof.
+rewrite /reduce => H; split; first smt(red256P).
+smt(red256_thrice).
+qed.
+
+
+
+(******************************************************************)
+(*                  ABSTRACT SPECIFICATIONS                       *)
+(******************************************************************)
+module ASpecFp = {
+  (* INTEGER OPS *)
+  proc eqn(a b: int) : bool = {
+    var r;
+    r <- (a=b);
+    return r;
+  }
+  proc eqn0(a: int) : bool = {
+    var r;
+    r <- (a=0);
+    return r;
+  }
+  proc addn(a b: int): bool * int = {
+    var c, r;
+    c <- modulusR <= (a+b);
+    r <- (a + b) %% modulusR;
+    return (c, r);
+  }
+  proc subn(a b: int): bool * int = {
+    var c, r;
+    c <- a < b;
+    r <- (a - b) %% modulusR;
+    return (c, r);
+  }
+  proc muln(a b: int): int = {
+    var r;
+    r <- a * b;
+    return r;
+  }
+  (* reduces "a \in [0..2^256[" into "x \in [0..P[" *)
+  proc freeze(a: int): zp = {
+    var r;
+    r <- inzp a;
+    return r;
+  }
+  proc set0n(): int = {
+    var r;
+    r <- 0;
+    return r;
+  }
+  proc ctseln(cond: bool, c a: int): int = {
+    var r;
+    r <- (if cond then a else c);
+    return r;
+  }
+  proc copyn(a: int): int = {
+    var r;
+    r <- a;
+    return r;
+  }
+  proc cminusP(a: int): int = {
+    var r;
+    r <- if a < P then a else a-P;
+    return r;
+  }
+  proc caddP(c: bool, a: int): int = {
+    var r;
+    r <- if c then (a+P)%%modulusR else a%%modulusR;
+    return r;
+  }
+  proc reduce(a: int): int = {
+    var r;
+    r <- reduce a;
+    return r;
+  }
+  (********************)
+  (* Finite Field Ops *)
+  (********************)
+  proc copym(a: zp): zp = {
+    var r;
+    r <- a;
+    return r;
+  }
+  proc set0m(): zp = {
+    var r;
+    r <- Zp.zero;
+    return r;
+  }
+  (* modular operations: finite field [Fp] *)
+  proc addm(a b: zp): zp = {
+    var r;
+    r <- a + b;
+    return r;
+  }
+  proc subm(a b: zp): zp = {
+    var r;
+    r <- a - b;
+    return r;
+  }
+  proc mulm(a b: zp): zp = {
+    var r;
+    r <- a * b;
+    return r;
+  }
+}.
+
+(******************************************************************)
+(*                  CONCRETE SPECIFICATIONS                       *)
+(******************************************************************)
+module CSpecFp = {
+ proc cminusP(a: int): int = {
+  var c, x, r;
+  (c, x) <@ ASpecFp.addn(a, 2^255 + 19);
+  r <@ ASpecFp.ctseln(c, a, x);
+  return r;
+ }
+ proc addm(a b: zp): int = {
+  var c, x, r;
+  (c, x) <@ ASpecFp.addn(asint a, asint b);
+  r <@ ASpecFp.cminusP(x);
+  return r;
+ }
+ proc caddP(c: bool, a: int): int = {
+  var x, r;
+  x <- ASpecFp.ctseln(c, 0, P);
+  (c, r) <@ ASpecFp.addn(a, x);
+  return r;
+ }
+ proc subm(a b: zp): int = {
+  var c, r, x;
+  (c, r) <@ ASpecFp.subn(asint a, asint b);
+  x <- ASpecFp.caddP(c, r);
+  return x;
+ }
+ proc freeze(a: int): int = {
+   var r;
+   r <@ ASpecFp.cminusP(a);
+   r <@ ASpecFp.cminusP(r);
+   return r;
+ }
+ proc mulm(a b: zp): int = {
+  var r, x;
+  r <@ ASpecFp.muln(asint a, asint b);
+  x <@ ASpecFp.reduce(r);
+  x <@ freeze(x);
+  return x;
+ }
+}.
+
+equiv cminusP_eq:
+ ASpecFp.cminusP ~ CSpecFp.cminusP: ={a} /\ a{2}<modulusR ==> ={res}.
+proof.
+proc; inline*; wp; skip => &1 &2.
+have ->: modulusR = 2^256 by rewrite R.bn_modulusE /= !mulrA expr0. 
+move=> [-> Ha] X.
+rewrite lerNgt if_neg.
+rewrite /X addrA ltP_overflow.
+case: (a{2} < P) => H; first done.
+rewrite redE 2://.
+split; last done. 
+smt().
+qed.
+
+equiv freeze_eq:
+ ASpecFp.freeze ~ CSpecFp.freeze: ={a} /\ 0<=a{2}<modulusR ==> asint res{1}=res{2}.
+proof.
+proc; inline*; wp; skip => &1 &2.
+have ->: modulusR = 2^256 by rewrite R.bn_modulusE /= !mulrA expr0. 
+move=> [-> [Ha1 Ha2]] /=.
+rewrite inzpK; case: (a{2} < P) => H0.
+ by rewrite modz_small /#.
+case: (a{2} - P < P) => H1.
+ rewrite {1}(_: a{2} = a{2} - P + P) 1:/# modzDr modz_small; last reflexivity.
+ by apply bound_abs => /#.
+rewrite (_: a{2} = a{2} - P - P + P + P) 1:/#.
+rewrite modzDr modzDr modz_small.
+apply bound_abs; split => *; first smt().
+move: Ha2 => /=; smt(pVal).
+smt().
+qed.
+
+
+equiv addm_eq:
+ ASpecFp.addm ~ CSpecFp.addm: ={a,b} ==> asint res{1}=res{2}.
+proof.
+proc; simplify.
++ inline*; wp; skip => /> &2.
+  have ->: (asint a{2} + asint b{2}) %% modulusR = (asint a{2} + asint b{2}).
+   rewrite modz_small. smt.
+   done.
+  case: (asint a{2} + asint b{2} < P) => H.
+   by rewrite addE modz_small; smt(rg_asint).
+  rewrite addE. smt. 
+qed.
+
+equiv caddP_eq:
+ ASpecFp.caddP ~ CSpecFp.caddP:
+  ={c,a} (*/\ 0<=a{2}<modulusR /\ (c{2} => modulusR < a{2}+P)*)
+  ==> ={res}.
+proof.
+proc; inline*; wp; skip => &1 &2 /=.
+have ->: modulusR = 2^256 by rewrite R.bn_modulusE /= !mulrA expr0. 
+move=> [-> ->] /=.
+case: (c{2}) => ?; first smt().
+by move=> /> *; rewrite modz_small /#.
+qed.
+
+equiv subm_eq:
+ ASpecFp.subm ~ CSpecFp.subm:
+  ={a,b} ==> asint res{1}=res{2}.
+proof.
+proc; simplify.
+inline*. wp; skip => />  &2.
+case: (asint a{2} < asint b{2} ) => /= H.
+ rewrite modzDml modz_small.
+  smt.
+ rewrite addE oppE modzDmr. smt.
+rewrite modz_small.
+ smt.
+rewrite addE oppE modzDmr. smt. 
+qed.
+
+equiv mulm_eq:
+ ASpecFp.mulm ~ CSpecFp.mulm: ={a,b} ==> asint res{1}=res{2}.
+proof.
+proc; simplify.
+transitivity {2}
+ { r <@ ASpecFp.muln(asint a, asint b); x <- reduce r; a <@ ASpecFp.freeze(x); }
+ ( ={a,b} ==> r{1}=a{2} )
+ ( ={a,b} ==> asint a{1} = x{2} ).
+ + by move=> /> &2; exists a{2} b{2} => /#.
+ + by move=> /> /#.
+ + inline*; wp; skip => /> &2.
+   apply asint_inj.
+   rewrite Zp.mulE inzpK. 
+   move: (reduceP (asint a{2}*asint b{2}) _).
+    move: (rg_asint a{2}) (rg_asint b{2}); smt(pVal).
+   smt().
+ + call freeze_eq.
+   inline*; wp; skip => &1 &2 [-> ->] /=.
+   move: (reduceP (asint a{2}*asint b{2}) _).
+    move: (rg_asint a{2}) (rg_asint b{2}); smt(pVal).
+   by rewrite R.bn_modulusE -exprM /= /#.
+qed.
